Cleaned example 1

Example.thy
@@ -5,99 +5,85 @@ begin
 text {* Goal: \<turnstile>\<^sub>P {x = 0} x := x+1 || x:= x+1 {x = 2} *}
 
 text {* 
+We add the auxiliary variables d1 and d2 (for done1 and done2).
+
 Annotated program: 
-  {x = 0, d1 = false, ...} (x := x+1, d1 := true) {x = x+1} 
+  {@{term "d1 = 0 \<and> (d2 = 0 \<longrightarrow> x = 0) \<and> (d2 = 1 \<longrightarrow> x = 1)"}} 
+  (x := x+1, d1 := true) 
+  {@{term "d1 = 1 \<and> (d2 = 0 \<longrightarrow> x = 1) \<and> (d2 = 1 \<longrightarrow> x = 2)"}} 
   || 
-  {x = 0, d2 = false, ...} (x:= x+1, d2 := true) {x = x+1} 
+  {@{term "d2 = 0 \<and> (d1 = 0 \<longrightarrow> x = 0) \<and> (d1 = 1 \<longrightarrow> x = 1)"}} 
+  (x:= x+1, d2 := true)
+  {@{term "d2 = 1 \<and> (d1 = 0 \<longrightarrow> x = 1) \<and> (d1 = 1 \<longrightarrow> x = 2)"}}
 
 Goal: \<turnstile>\<^sub>P {x = 0, d1 = false, d2 = false} x := x+1 || x:= x+1 {x = 2}
 *}
 
-abbreviation pre1 :: "assn" where "pre1 \<equiv> \<lambda>s. s ''d1'' = 0 \<and> (s ''d2'' = 0 \<longrightarrow> s ''x'' = 0) \<and> (s ''d2'' = 1 \<longrightarrow> s ''x'' = 1)"
-abbreviation pre2  :: "assn" where "pre2 \<equiv> \<lambda>s. s ''d2'' = 0 \<and> (s ''d1'' = 0 \<longrightarrow> s ''x'' = 0) \<and> (s ''d1'' = 1 \<longrightarrow> s ''x'' = 1)"
-abbreviation post1 :: "assn" where "post1 \<equiv> \<lambda>s. s ''d1'' = 1 \<and> (s ''d2'' = 0 \<longrightarrow> s ''x'' = 1) \<and> (s ''d2'' = 1 \<longrightarrow> s ''x'' = 2)"
-abbreviation post2  :: "assn" where "post2 \<equiv> \<lambda>s. s ''d2'' = 1 \<and> (s ''d1'' = 0 \<longrightarrow> s ''x'' = 1) \<and> (s ''d1'' = 1 \<longrightarrow> s ''x'' = 2)"
+abbreviation pre1 :: "assn" where 
+  "pre1 \<equiv> \<lambda>s. s ''d1'' = 0 \<and> (s ''d2'' = 0 \<longrightarrow> s ''x'' = 0) \<and> (s ''d2'' = 1 \<longrightarrow> s ''x'' = 1)"
+abbreviation pre2  :: "assn" where 
+  "pre2 \<equiv> \<lambda>s. s ''d2'' = 0 \<and> (s ''d1'' = 0 \<longrightarrow> s ''x'' = 0) \<and> (s ''d1'' = 1 \<longrightarrow> s ''x'' = 1)"
+abbreviation post1 :: "assn" where 
+  "post1 \<equiv> \<lambda>s. s ''d1'' = 1 \<and> (s ''d2'' = 0 \<longrightarrow> s ''x'' = 1) \<and> (s ''d2'' = 1 \<longrightarrow> s ''x'' = 2)"
+abbreviation post2  :: "assn" where 
+  "post2 \<equiv> \<lambda>s. s ''d2'' = 1 \<and> (s ''d1'' = 0 \<longrightarrow> s ''x'' = 1) \<and> (s ''d1'' = 1 \<longrightarrow> s ''x'' = 2)"
 
-abbreviation plus11  :: "state \<Rightarrow> state" where "plus11 \<equiv> \<lambda>s. s(''x'' := s ''x'' + 1, ''d1'' := 1)"
-abbreviation plus12  :: "state \<Rightarrow> state" where "plus12 \<equiv> \<lambda>s. s(''x'' :=  s ''x'' + 1, ''d2'' := 1)"
+abbreviation plus11  :: "state \<Rightarrow> state" where 
+  "plus11 \<equiv> \<lambda>s. s(''x'' := s ''x'' + 1, ''d1'' := 1)"
+abbreviation plus12  :: "state \<Rightarrow> state" where 
+  "plus12 \<equiv> \<lambda>s. s(''x'' :=  s ''x'' + 1, ''d2'' := 1)"
 
 abbreviation "C2 \<equiv> ABasic pre2 (plus12)"
+abbreviation "C1 \<equiv> ABasic pre1 (plus11)"
 
-abbreviation Ts :: "((acom option \<times> assn) list)" where "Ts \<equiv> [((Some (ABasic pre1 (plus11))), post1), ((Some (ABasic pre2 (plus12))), post2)]"
-
-lemma "\<forall>(R, r) \<in> (atomics C2). \<Turnstile>\<^sub>t\<^sub>r {\<lambda>s. post1 s \<and> R s} r {post1}"
-apply auto oops
+abbreviation Ts :: "((acom option \<times> assn) list)" where 
+  "Ts \<equiv> [(Some C1, post1), (Some C2, post2)]"
 
 subsubsection{* Proof by Hoare Logic *}
 
-(* declare [[show_types]] *)
-
 lemma "\<turnstile>\<^sub>P {\<lambda>s. s ''x'' = 0 \<and> s ''d1'' = 0 \<and> s ''d2'' = 0} Parallel Ts {\<lambda>s. s ''x'' = 2}"
 proof -
-  have Ind:"Index Ts = {0, Suc 0}"
+  text {* We will use the rule Parallel of the definition of @{term "hoare_par"}} to obtain 
+    @{term "\<turnstile>\<^sub>P {\<lambda> s . pre1 s \<and> pre2 s} (Parallel Ts) {\<lambda>s. post1 s \<and> post2 s}"}.
+    We will finally reach our goal by strengthening the precondition and weakening the postcondition *}
+  text {* An auxiliary lemma *}
+  have index:"Index Ts = {0,1::nat}"
   proof -
-    have "length Ts = 2" by simp
-    hence "Index2 Ts = {0, Suc 0}" by auto
-    thus ?thesis using Index_Equal by blast
+    have "Index Ts = Index2 Ts" using Index_Equal by blast
+    also have "... = {0,1::nat}" by auto
+    finally show ?thesis by auto
   qed
-  obtain C1::acom and Q1::assn where 0:"(Ts!0) = (Some C1, Q1)" by simp
-  obtain C2::acom and Q2::assn where 1:"(Ts!1) = (Some C2, Q2)" by simp
-  have "\<turnstile> C1 {Q1}" and "\<turnstile> C2 {Q2}" using 0 1 by auto
-  hence 3:"(\<forall>i \<in> Index Ts. \<exists>(c::acom) Q. (Ts!i) = (Some c, Q) \<and> (\<turnstile> c {Q}))" by (metis (no_types, lifting) 0 1 Ind One_nat_def insertE singletonD)
-  have "INTERFREE Ts"
+  have "\<turnstile>\<^sub>P {\<lambda> s . pre1 s \<and> pre2 s} (Parallel Ts) {\<lambda>s. post1 s \<and> post2 s}"
   proof -
-    have "(\<forall>(R, r) \<in> (atomics C2). \<Turnstile>\<^sub>t\<^sub>r {\<lambda>s. Q1 s \<and> R s} r {Q1} \<and> (\<forall>P \<in> (assertions C1).\<Turnstile>\<^sub>t\<^sub>r {\<lambda>s. P s \<and> R s} r {P}))"
+    text {* We establish the two premises of the rule Parallel separately *}
+    have premise1:"(\<forall>i \<in> Index Ts. \<exists>(c::acom) Q. (Ts!i) = (Some c, Q) \<and> (\<turnstile> c {Q}))" 
+      using index by simp 
+    have premise2:"INTERFREE Ts"
     proof -
-      have "\<forall>(R, r) \<in> (atomics C2). \<Turnstile>\<^sub>t\<^sub>r {\<lambda>s. Q1 s \<and> R s} r {Q1}"
+      have "interfree (com(Ts ! 0), post(Ts ! 0), com(Ts!1))"
       proof -
-        have "\<turnstile>\<^sub>t\<^sub>r {\<lambda>s. Q1 s \<and> pre2 s} Basic plus12 {Q1}" using 0 by auto
-        hence "\<Turnstile>\<^sub>t\<^sub>r {\<lambda>s. Q1 s \<and> pre2 s} Basic plus12 {Q1}" using hoare_sound_tr by blast
-        thus ?thesis using 1 hoare_sound_tr by auto
+        have "\<turnstile>\<^sub>t\<^sub>r {\<lambda>s. post1 s \<and> pre2 s} Basic plus12 {post1}" by auto
+        moreover have "\<turnstile>\<^sub>t\<^sub>r {\<lambda>s. pre1 s \<and> pre2 s} Basic plus12 {pre1}" by auto
+        ultimately show ?thesis using hoare_sound_tr by auto
       qed
       moreover
-      have "\<forall>(R, r) \<in> (atomics C2).(\<forall>P \<in> (assertions C1).\<Turnstile>\<^sub>t\<^sub>r {\<lambda>s. P s \<and> R s} r {P})"
+      have "interfree(com(Ts ! 1), post(Ts ! 1), com(Ts!0))"
       proof -
-        have "vc_tr (Basic plus12) pre1" using vc_tr.simps(1) by blast
-        hence "\<turnstile>\<^sub>t\<^sub>r {\<lambda>s. pre1 s \<and> pre2 s} Basic plus12 {pre1}" using 0 by auto
-        hence "\<Turnstile>\<^sub>t\<^sub>r {\<lambda>s. pre1 s \<and> pre2 s} Basic plus12 {pre1}" using hoare_sound_tr by blast
-        thus ?thesis using 0 1 by auto
+        have "\<turnstile>\<^sub>t\<^sub>r {\<lambda>s. post2 s \<and> pre1 s} Basic plus11 {post2}" by auto
+        moreover have "\<turnstile>\<^sub>t\<^sub>r {\<lambda>s. pre2 s \<and> pre1 s} Basic plus11 {pre2}" by auto
+        ultimately show ?thesis using hoare_sound_tr  by auto
       qed
-      ultimately show ?thesis by blast
+      ultimately show ?thesis using index INTERFREE_def by auto
     qed
-    hence 5:"interfree(Some C1, Q1, Some C2)" using interfree.simps(3) by presburger
-    have "(\<forall>(R, r) \<in> (atomics C1). \<Turnstile>\<^sub>t\<^sub>r {\<lambda>s. Q2 s \<and> R s} r {Q2} 
-      \<and> (\<forall>P \<in> (assertions C2).\<Turnstile>\<^sub>t\<^sub>r {\<lambda>s. P s \<and> R s} r {P}))"
-    proof -
-      have "\<forall>(R, r) \<in> (atomics C1). \<Turnstile>\<^sub>t\<^sub>r {\<lambda>s. Q2 s \<and> R s} r {Q2}"
-      proof -
-        have "vc_tr (Basic plus11) Q2" using vc_tr.simps(1) by blast
-        hence "\<turnstile>\<^sub>t\<^sub>r {\<lambda>s. Q2 s \<and> pre1 s} Basic plus11 {Q2}" using 1 by auto
-        hence "\<Turnstile>\<^sub>t\<^sub>r {\<lambda>s. Q2 s \<and> pre1 s} Basic plus11 {Q2}" using hoare_sound_tr by blast
-        thus ?thesis using 0 hoare_sound_tr by auto
-      qed
-      moreover
-      have "\<forall>(R, r) \<in> (atomics C1).(\<forall>P \<in> (assertions C2).\<Turnstile>\<^sub>t\<^sub>r {\<lambda>s. P s \<and> R s} r {P})"
-      proof -
-        have "vc_tr (Basic plus11) pre2" using vc_tr.simps(1) by blast
-        hence "\<turnstile>\<^sub>t\<^sub>r {\<lambda>s. pre2 s \<and> pre1 s} Basic plus11 {pre2}" using 0 by auto
-        hence "\<Turnstile>\<^sub>t\<^sub>r {\<lambda>s. pre2 s \<and> pre1 s} Basic plus11 {pre2}" using hoare_sound_tr by blast
-        thus ?thesis using 0 1 by auto
-      qed
-      ultimately show ?thesis by blast
-    qed
-    hence "interfree(Some C2, Q2, Some C1)" using interfree.simps(3) by presburger
-    hence "\<forall>i \<in> Index Ts. \<forall>j \<in> Index Ts. i \<noteq> j \<longrightarrow> interfree(com(Ts ! i), post(Ts ! i), com(Ts!j))" using Ind 0 1 5
-      by (smt One_nat_def Proof_Par.com.simps(1) insertE post.simps singletonD)
-    thus ?thesis  using INTERFREE_def by blast
+    text {* Then we establish the pre and post used in the Parallel rule *}
+    have pre:"(\<lambda> s . \<forall>i \<in> Index Ts. (pre (the (com(Ts!i)))) s) = (\<lambda> s . pre1 s \<and> pre2 s)" 
+      using index by force 
+    have post:"(\<lambda> s . \<forall>i \<in> Index Ts. (post (Ts!i)) s) = (\<lambda>s. post1 s \<and> post2 s)"
+      using index  by force 
+    from premise1 premise2 pre post show ?thesis using Parallel[where ?Ts="Ts"] index by auto
   qed
-  hence 7:"vc_par (Parallel Ts) (\<lambda> s . \<forall>i \<in> Index Ts. (post (Ts!i)) s)" using Ind 0 1 3 by simp
-  have "\<forall>s. (\<lambda>s. \<forall>i \<in> Index Ts. (post (Ts!i)) s) s \<longrightarrow> (\<lambda>s. s ''x'' = 2) s"
-    by (smt Ind insertI1 insert_commute nth_Cons_0 nth_Cons_Suc post.simps) 
-  hence 8:"vc_par (Parallel Ts) (\<lambda>s. s ''x'' = 2)" using 7 vc_mono_par by smt
-  hence 9:"\<turnstile>\<^sub>P {\<lambda> s . \<forall>i \<in> Index Ts. (pre (the (com(Ts!i)))) s} (Parallel Ts) {\<lambda>s. s ''x'' = 2}" using pre_par.simps(1) vc_sound_par' by presburger
-  have "\<forall>s. (\<lambda>s. s ''x'' = 0 \<and> s ''d1'' = 0 \<and> s ''d2'' = 0) s \<longrightarrow> (\<lambda> s . \<forall>i \<in> Index Ts. (pre (the (com(Ts!i)))) s) s"
-    by (smt Ind Proof_Par.com.simps(1) insertE nth_Cons_0 nth_Cons_Suc option.sel pre.simps(1) singletonD)
-  thus ?thesis by (smt 8 9 pre_par.simps(1) vc_sound_par')
+  thus ?thesis using ParConseq
+    by smt
 qed
 
 end
